deps/poulet4/lib/P4automata/Examples/SimpleLoop.v
@@ -86,6 +86,7 @@ End Loop.
 (* Lemma prebisim_loop:
   pre_bisimulation (Sum.sum Loop.aut Loop.aut)
                    (WPSymLeap.wp (H:=_))
+                   (separated _ _ _ (Sum.sum Loop.aut Loop.aut))
                    nil
                    (mk_init 10 (Sum.sum Loop.aut Loop.aut) Loop.Start Loop.Start)
                    (inl (inl Loop.Start), [], [])
@@ -94,45 +95,7 @@ Proof.
   set (rel0 := mk_init 10 (Sum.sum Loop.aut Loop.aut) Loop.Start Loop.Start).
   cbv in rel0.
   subst rel0.
-  solve_bisim'.
-  solve_bisim'.
-  Notation "x == y" := (BREq x y) (at level 40).
-  Notation "side . x" := (BEHdr _ side x) (at level 40).
-  Notation "⟪ x ⟫" := (HRVar x) (at level 40).
-  Notation "⦃ x ⦄" := (BELit _ _ x) (at level 30).
-  Notation "x ∨ y" := (BROr x y) (at level 30).
-  simpl.
-  solve_bisim'.
-  solve_bisim'.
-  solve_bisim'.
-  solve_bisim'.
-  solve_bisim'.
-  solve_bisim'.
-  apply PreBisimulationSkip;
-   [ intros; cbn in *; unfold interp_conf_rel, interp_store_rel, interp_conf_state, interp_state_template in *;
-      simpl in * |].
-  {
-    simpl.
-    subst.
-    intros.
-    destruct valu as [[_ [b1 ?]] [b2 ?]].
-    intuition.
-    destruct q1 as [[? ?] ?], q2 as [[? ?] ?]; simpl in *.
-    destruct l, l0; simpl in *; try solve [simpl in *; congruence].
-  }
-  apply PreBisimulationSkip;
-   [ intros; cbn in *; unfold interp_conf_rel, interp_store_rel, interp_conf_state, interp_state_template in *;
-      simpl in * |].
-  {
-    simpl.
-    subst.
-    intros.
-    destruct valu as [[_ [b1 ?]] [b2 ?]].
-    intuition.
-    destruct q1 as [[? ?] ?], q2 as [[? ?] ?]; simpl in *.
-    destruct l, l0; simpl in *; try solve [simpl in *; congruence].
-  }
-  solve_bisim'.
+  repeat solve_bisim'.
   cbv in *.
   intuition (try congruence).
 Time Qed. *)
